Xserver reworked to better map to network

FSharpNemlogIn/FStarWrapper/Program.fs
@@ -3,17 +3,11 @@ open System.Security.Cryptography
 open Network
 open CryptoTest
 
-let rec StartListen() =
-    xServer.server "sp" "idp"
-    let key = Console.ReadKey ()
-    match key.KeyChar with
-    | 'x' -> ()
-    | _ -> StartListen()
-
-
 [<EntryPoint>]
 let main argv = 
   
-  let x = X.GenKeys("some important principal")
+  let s = X.test1 "h"
+
+
   let key = Console.Read ()
   0 // return an integer exit code
