FSharpNemlogIn/RuntimeExtention/Crypto.fs
@@ -1,0 +1,52 @@
+﻿module Crypto
+
+open System.Security.Cryptography
+open System.Text
+open System
+open System.IO
+
+let GetEncoder = new ASCIIEncoding()
+
+let GetHashProvicer = new SHA1CryptoServiceProvider()
+
+let GetCryptoProvider = new RSACryptoServiceProvider()
+
+let WriteKeyToFile (filename:string) (key:string) = 
+    // save to file
+    let fn = filename.Replace("://", "-")
+    let file = File.CreateText(fn)
+    file.Write key |>  file.Close
+
+let KeyGenExt prin : Prims.DepTuple<Protocol.pubkey,Protocol.privkey> = 
+    let cspParams = new CspParameters()
+    cspParams.ProviderType <- 1
+    cspParams.Flags <- CspProviderFlags.UseArchivableKey
+    cspParams.KeyNumber <- int KeyNumber.Exchange
+    let rsaProvicer = GetCryptoProvider
+
+    // Export Public Key
+    let pubkey = Protocol.pubkey(0,rsaProvicer.ToXmlString false)
+
+    // Export private key
+    let privkey = Protocol.privkey(0,rsaProvicer.ToXmlString true)
+
+    new Prims.DconDepTuple<Protocol.pubkey,Protocol.privkey>(pubkey, privkey) :> Prims.DepTuple<Protocol.pubkey,Protocol.privkey>
+
+let SignMessage (prin:string) (key:string) (msg:string) : string = 
+    let ByteConverter = GetEncoder
+    let msgData = ByteConverter.GetBytes(msg)
+    let alg = GetCryptoProvider
+    alg.FromXmlString key
+    let signedData = alg.SignData(msgData, GetHashProvicer)
+
+    Convert.ToBase64String(signedData)
+
+let ValidateMessage (prin:string) (key:string) (msg:string) (signature:string) : bool = 
+    let ByteConverter = GetEncoder
+    let dataToVerify = ByteConverter.GetBytes msg
+    let sign = Convert.FromBase64String signature
+    let alg = GetCryptoProvider
+    alg.FromXmlString key
+
+    alg.VerifyData(dataToVerify, GetHashProvicer, sign)
+
