Protocol/SAMLProtocol.fst
@@ -1,8 +1,8 @@
 module Protocol
 
 type prin = string
-type pubkey :: prin => string 
-type privkey :: prin => string
+type pubkey :: prin => *
+type privkey :: prin => *
 type dsig = string
 type resource = bytes
 type uri = string
@@ -59,16 +59,4 @@ extern reference Crypto {language="F#";
 extern Crypto val KeyGenExt: p:prin
           -> (pubkey p * privkey p)
 
-
-(*Saml functions*)
-extern reference Saml {language="F#";
-            dll="Saml";
-            namespace="";
-            classname="Saml"}
-
-extern Saml val CreateAuthnRequest: issuer:prin -> destination:prin -> samlmessage
-extern Saml val CreateChallenge: prin -> nonce
-extern Saml val CreateSamlAssertion: user:string -> issuer:prin -> destination:prin -> assertion
-extern Saml val CreateSamlResponse: issuer:prin -> destination:prin -> assertion -> samlmessage
-extern Saml val CreateSamlFailedResponse: issuer:prin -> destination:prin -> SamlStatus -> samlmessage
 
