Protocol/Crypto.fst
@@ -1,0 +1,35 @@
+module Crypto
+
+open Protocol
+
+val Keygen:  p:prin
+          -> (pubkey p * privkey p)
+
+val Sign:  p:prin
+        -> privkey p
+        -> msg:samlmessage{Log p msg}
+        -> dsig
+
+val VerifySignature: p:prin
+        -> pubkey p 
+        -> msg:samlmessage
+        -> dsig
+        -> b:bool{b=true ==> Log p msg}
+
+val AuthenticateUser: user:string
+        -> password:string
+        -> challenge:nonce
+        -> b:bool{b=true ==> Log2 user password challenge}
+
+(*val Encrypt: ...
+
+val Decrypt: ...*)
+
+(*Crypto functions*)
+extern reference Crypto {language="F#";
+            dll="Crypto";
+            namespace="";
+            classname="Crypto"}
+
+extern Crypto val KeyGenExt: p:prin
+          -> (pubkey p * privkey p)
