Protocol/DummyNetwork.fst
@@ -1,0 +1,37 @@
+module DummyNetwork
+
+open Lib
+open Protocol
+
+val SendResponse: prin -> list string -> string -> bool
+let SendResponse prin cookies messagebody =
+	println "Response to prin:";
+	println prin;
+	println "cookies:";
+	printlist cookies;
+	println "messagebody:";
+	println messagebody
+
+val SendRequest: uri -> list string -> string -> bool
+let SendRequest dest cookies messagebody =
+	println "MessageDestination:";
+	println dest;
+	println "cookies:";
+	printlist cookies;
+	println "messagebody:";
+	println messagebody
+
+val RecieveResponse: prin -> (int *string * list string)
+let RecieveResponse prin =
+	let status = 200 in
+	let body = "The message" in 
+	let cookies = ["cookie1=someval"; "cookie2=somotherval"] in
+	(status, body, cookies)
+
+val RecieveRequest: prin -> (string * string * string * list string)
+let RecieveRequest prin =
+	let verb = "GET" in
+	let url = "https://sp.dk?samlMessage=SGVyZSBpcyBhIHNhbWwgbWVzc2FnZQ==" in (*Here is a saml message*)
+	let body = "The message if post" in 
+	let cookies = ["cookie1=someval"; "cookie2=somotherval"] in
+	(verb, url, body, cookies)
