Protocol/Lib.fst
@@ -1,0 +1,39 @@
+module Lib
+
+val ConcatList: string -> list string -> string
+let ConcatList sep l = match l with 
+  | [] -> ""
+  | hd::tl -> 
+      let tl = ConcatList sep tl in
+        if tl="" then hd
+        else Concat (Concat hd sep) tl
+
+val Concatkv: string -> string -> string -> string
+let Concatkv k sep v = 
+	let ks = Concat k sep in
+	Concat ks v
+
+val printlist: list string -> unit
+let printlist l = match l with
+	| [] -> ()
+	| hd::tl -> println hd;
+		printlist tl
+
+val getStrInList: list string -> string -> string
+let getStrInList l str = match l with
+	| [] -> ""
+	| hd::tl ->
+		if strStartsWith hd str then hd
+		else getStrInList tl str
+
+val isEmptyStr: string -> bool
+let isEmptyStr str = match str with
+      | "" -> false
+      | _ -> true
+
+val getListItem: list string -> string -> option string
+let getListItem l item = match l with
+	| [] -> None
+	| hd::tl -> 
+		if strStartsWith hd item then Some hd
+		else getListItem tl item
