Protocol/Network.fst
@@ -1,0 +1,48 @@
+module Network
+
+open Lib
+open Protocol
+
+(*Dummy implementation of actual networking*)
+open DummyNetwork
+
+(*This is the reference to the implementation in F#
+	This ic commented out for now to avoid struggeling with interop
+extern reference Network {language="F#";
+						dll="RuntimeExtention";
+						namespace="";
+						classname="Network"}
+extern Network val SendResponse: prin -> list string -> string -> bool
+extern Network val SendRequest: uri -> list string -> string -> bool
+extern Network val RecieveResponse: prin -> (int *string * list string)
+extern Network val RecieveRequest: prin -> (string * string * string * list string)
+*)
+
+type HttpMessage =
+	| Get: prin -> string -> list string -> list string -> HttpMessage
+ 	| Post: prin -> list string -> list string -> HttpMessage
+ 	| Redirect: prin -> string -> list string -> list string -> HttpMessage
+	| Response: int -> body:string -> HttpMessage
+
+val buildDestination: string -> list string -> string
+let buildDestination url params =
+	 let paramStr = ConcatList ";" params in
+	 Concatkv url "?" paramStr
+
+val Send: HttpMessage -> unit
+let Send message =
+	match message with
+	| Get (prin,url,params,cookies) -> 
+		let dest = buildDestination url params in
+		SendRequest dest cookies "hello";()
+	| _ -> println "Not yet implemented";
+		()
+
+val Recieve: prin -> HttpMessage
+let Recieve client =
+	let (verb,url,body,cookies) = RecieveRequest client in
+	match verb with
+	| "GET" -> 
+		let params = ["here query=params should be"] in
+		Get client url params cookies
+	| _ -> Response 400 "failed"
