Protocol/Protocol.fst
@@ -1,0 +1,14 @@
+module Protocol
+
+type prin = string
+type uri = string
+type pubkey :: prin => *
+type privkey :: prin => *
+type dsig = string
+type samlmessage = string
+type nonce = string (*How to secure uniqueness? P-kind?*)
+type assertion = string (*Shhould be ecrypted*)
+
+(*Verification*)
+type Log :: prin => samlmessage => E
+type Log2 :: string => string => nonce => E
