Protocol/Saml.fst
@@ -1,0 +1,30 @@
+module Saml
+
+open Protocol
+open Network
+
+
+type SamlStatus =
+  | Success: SamlStatus
+  | Requester: SamlStatus
+  | Responder: SamlStatus
+
+(*Saml functions*)
+extern reference Saml {language="F#";
+            dll="Saml";
+            namespace="";
+            classname="Saml"}
+
+extern Saml val CreateAuthnRequest: issuer:prin -> destination:prin -> samlmessage
+extern Saml val CreateChallenge: prin -> nonce
+extern Saml val CreateSamlAssertion: user:string -> issuer:prin -> destination:prin -> assertion
+extern Saml val CreateSamlResponse: issuer:prin -> destination:prin -> assertion -> samlmessage
+extern Saml val CreateSamlFailedResponse: issuer:prin -> destination:prin -> SamlStatus -> samlmessage
+
+val CreateRedirectResponse: prin -> samlmessage -> dsig -> string -> HttpMessage
+let CreateRedirectResponse prin msg sig relay =
+      (*Base64 encode all params*)
+      let params = [msg; sig; relay] in
+      let cookies = [relay] in
+      let resp = Redirect prin prin params cookies in 
+      resp
